{
  "@context": {
    "schema": "http://schema.org/",
    "bs": "https://bioschemas.org/terms/",
    "codemeta": "https://w3id.org/codemeta/",
    "rdf": "http://www.w3.org/1999/02/22-rdf-syntax-ns#",
    "rdfs": "http://www.w3.org/2000/01/rdf-schema#",
    "maSMP:": "https://discovery.biothings.io/view/maSMP/",
    "@dateModified": "2023-11-30"
  },
  "@graph": [
    {
      "@id": "schema:programmingLanguage",
      "@type": "rdf:Property",
      "rdfs:comment": "The computer programming language.",
      "rdfs:label": "programmingLabel",
      "text": "Java"
    },
    {
      "@id": "schema:version",
      "@type": "rdf:Property",
      "rdfs:comment": "The version of the CreativeWork embodied by a specified resource.",
      "rdfs:label": "version"
    },
    {
      "@id": "schema:citation",
      "@type": "rdf:Property",
      "rdfs:comment": "A citation or reference to another creative work, such as another publication, web page, scholarly article, etc. Values expected to be one of these types.",
      "rdfs:label": "citation"
    },
    {
      "@id": "schema:contributor",
      "@type": "rdf:Property",
      "rdfs:comment": "Contributors.",
      "rdfs:label": "contributor"
    },
    {
      "@id": "schema:description",
      "@type": "rdf:Property",
      "rdfs:comment": "A description of the item..",
      "rdfs:label": "description",
      "text": " * License and Copyright: FedoraGSearch is subject to the same open source \n * license as the Fedora Repository System at www.fedora-commons.org\n * Copyright 2006, 2007, 2008 by The Technical University of Denmark.\n * All rights reserved.\n \n The FedoraGSearch development is funded by \n \n     DEFF, Denmark's Electronic Research Library, http://www.deff.dk .\n     \nThe developer is Gert Schmeltz Pedersen, gsp@dtic.dtu.dk, at \nthe Technical Information Center of Denmark at the Technical University of Denmark. \nContact in the Fedora core developer team is Chris Wilper, cwilper@fedora-commons.org . \nVersion 2.0 was released in February 2008, with new features requested by users.\nThe main and overall aim is to exploit more features of Lucene.\nIt works with Fedora version 2.2.1. \nVersion 2.1 was released in April 2008, updating GSearch to work with Fedora 3.0\nand taking advantage of Fedora's new messaging capability for index updates. \nThe new features in Version 2.2: \n- Fedora 3.1 compatibility\n- Lucene 2.4.0 compatibility\n- Solr 1.3.0 compatibility\n- For the lucene plugin: Search result filtering by access constraints, as defined by XACML policies,\n  in order to show only those search hits that the user is actually permitted to read. \nThe new features in Version 2.1: \n- Update listener which uses the Fedora messaging client to listen for \n  updates being performed through API-M. These update messages contain the \n  information needed to perform index updates, thereby keeping GSearch\n  up-to-date with the Fedora repository. \nThe new features in Version 2.0: \n- Added easier configuration, so that you need only edit one file\n  with property values, then run it with ant.\n\t\t\t\t    \n- Added a sortFields parameter to gfindObjects for Lucene, sorting\n  search results as specified, exploiting Lucene classes for sorting.\n  \n- Added optimize options for Lucene indexing. The mergeFactor and maxBufferedDocs\n  properties will affect performance as explained in the Lucene documentation.\n  The optimize action of the updateIndex operation will perform the Lucene method \n  call IndexWriter.optimize(), which merges all segments together into a single segment, \n  optimizing an index for search. The optimize() is no longer called after each updateIndex. \n- Added parameters to the indexDocXslt parameter of the updateIndex operation,\n  enabling the transfer of param values into the indexing stylesheet.\n\t\t\t\t    \n- Added untokenizedFields property to Lucene index.properties files.\n  Adding the property with a list of all untokenized fields will\n  ensure that they all select the appropriate analyzer.\n\t\t\t\t    \n- Added properties snippetBegin and snippetEnd, making highlight code configurable.\n\t\t\t\t    \n- Added property for custom URIResolver used by xslt transformers\n  for basic authorization and SSL,\n  see the example dk.defxws.fedoragsearch.server.URIResolverImpl class.\n\t\t\t\t\t\n- Removed encoding of special characters in indexFields.\n  Snippets now show special characters without modification.\n  Indexes should be reindexed. \n"
    },
    {
      "@id": "schema:identifier",
      "@type": "rdf:Property",
      "rdfs:comment": "The identifier property represents any kind of identifier for any kind of Thing, such as ISBNs, GTIN codes, UUIDs etc. Schema.org provides dedicated properties for representing many of these, either as textual strings or as URL (URI) links. See background notes for more details.",
      "rdfs:label": "identifier"
    },
    {
      "@id": "schema:keywords",
      "@type": "rdf:Property",
      "rdfs:comment": "Keywords or tags used to describe some item. Multiple textual entries in a keywords list are typically delimited by commas, or by repeating the property.",
      "rdfs:label": "keywords",
      "text": ""
    },
    {
      "@id": "schema:license",
      "@type": "rdf:Property",
      "rdfs:comment": "license",
      "rdfs:label": "license",
      "url": "Copyright (c) 2003-2005, www.pdfbox.org\nAll rights reserved.\n\nRedistribution and use in source and binary forms, with or without\nmodification, are permitted provided that the following conditions are met:\n\n1. Redistributions of source code must retain the above copyright notice,\n   this list of conditions and the following disclaimer.\n2. Redistributions in binary form must reproduce the above copyright notice,\n   this list of conditions and the following disclaimer in the documentation\n   and/or other materials provided with the distribution.\n3. Neither the name of pdfbox; nor the names of its\n   contributors may be used to endorse or promote products derived from this\n   software without specific prior written permission.\n\nTHIS SOFTWARE IS PROVIDED BY THE COPYRIGHT HOLDERS AND CONTRIBUTORS \"AS IS\"\nAND ANY EXPRESS OR IMPLIED WARRANTIES, INCLUDING, BUT NOT LIMITED TO, THE\nIMPLIED WARRANTIES OF MERCHANTABILITY AND FITNESS FOR A PARTICULAR PURPOSE ARE\nDISCLAIMED.  IN NO EVENT SHALL THE REGENTS OR CONTRIBUTORS BE LIABLE FOR ANY\nDIRECT, INDIRECT, INCIDENTAL, SPECIAL, EXEMPLARY, OR CONSEQUENTIAL DAMAGES\n(INCLUDING, BUT NOT LIMITED TO, PROCUREMENT OF SUBSTITUTE GOODS OR SERVICES;\nLOSS OF USE, DATA, OR PROFITS; OR BUSINESS INTERRUPTION) HOWEVER CAUSED AND ON\nANY THEORY OF LIABILITY, WHETHER IN CONTRACT, STRICT LIABILITY, OR TORT\n(INCLUDING NEGLIGENCE OR OTHERWISE) ARISING IN ANY WAY OUT OF THE USE OF THIS\nSOFTWARE, EVEN IF ADVISED OF THE POSSIBILITY OF SUCH DAMAGE."
    },
    {
      "@id": "schema:maintainer",
      "@type": "rdf:Property",
      "rdfs:comment": "maintainer",
      "rdfs:label": "maintainer"
    },
    {
      "@id": "schema:name",
      "@type": "rdf:Property",
      "rdfs:comment": "The name of the item.",
      "rdfs:label": "name",
      "text": "fedora-genericsearch-2.2"
    },
    {
      "@id": "codemata:referencePublication",
      "@type": "rdf:Property",
      "rdfs:comment": "An academic publication related to the software.",
      "rdfs:label": "referencePublication"
    },
    {
      "@id": "schema:installURL",
      "@type": "rdf:Property",
      "rdfs:comment": "URL at which the app may be installed, if different from the URL of the item.",
      "rdfs:label": "installURL",
      "url": "https://github.com/MPDL/fedora-genericsearch-2.2/releases"
    },
    {
      "@id": "bs:input",
      "@type": "rdf:Property",
      "schema:domainIncludes": [
        {
          "@id": "maSMP:SoftwareSourceCode"
        },
        {
          "@id": "maSMP:SoftwareApplication"
        }
      ],
      "schema:rangeIncludes": {
        "@id": "bs:FormalParameter"
      },
      "rdfs:comment": "An input required to use the computational workflow (eg. Excel spreadsheet, BAM file).",
      "rdfs:label": "input"
    },
    {
      "@id": "bs:output",
      "@type": "rdf:Property",
      "schema:domainIncludes": [
        {
          "@id": "maSMP:SoftwareSourceCode"
        },
        {
          "@id": "maSMP:SoftwareApplication"
        }
      ],
      "schema:rangeIncludes": {
        "@id": "bs:FormalParameter"
      },
      "rdfs:comment": "An output produced by the computational workflow (or software).",
      "rdfs:label": "output"
    },
    {
      "@id": "codemeta:readme",
      "@type": "rdf:Property",
      "schema:domainIncludes": [
        {
          "@id": "maSMP:SoftwareSourceCode"
        },
        {
          "@id": "maSMP:SoftwareApplication"
        }
      ],
      "schema:rangeIncludes": {
        "@id": "schema:URL"
      },
      "rdfs:comment": "Link to this software Readme file. Property defined in the [Codemeta terms](https://codemeta.github.io/terms/).",
      "rdfs:label": "readme"
    },
    {
      "@id": "schema:operatingSystem",
      "@type": "rdf:Property",
      "schema:domainIncludes": {
        "@id": "maSMP:SoftwareRunAction"
      },
      "schema:rangeIncludes": {
        "@id": "schema:Text"
      },
      "rdfs:comment": "If the running was done by a direct execution (rather than via a container), indicate the operating system.",
      "rdfs:label": "operatingSystem"
    },
    {
      "@id": "schema:processorRequirements",
      "@type": "rdf:Property",
      "schema:domainIncludes": {
        "@id": "maSMP:SoftwareRunAction"
      },
      "schema:rangeIncludes": {
        "@id": "schema:Text"
      },
      "rdfs:comment": "If the running was done by a direct execution (rather than via a container), indicate the processor specification.",
      "rdfs:label": "processorRequirements"
    },
    {
      "@id": "schema:runtimePlatform",
      "@type": "rdf:Property",
      "schema:domainIncludes": {
        "@id": "maSMP:SoftwareRunAction"
      },
      "schema:rangeIncludes": {
        "@id": "schema:Text"
      },
      "rdfs:comment": "If the running was done by a direct execution (rather than via a container), indicate the runtime platform.",
      "rdfs:label": "runtimePlatform"
    },
    {
      "@id": "maSMP:SoftwareApplication",
      "@type": "rdfs:Class",
      "rdfs:comment": "Extension of schema:SoftwareApplication adding properties corresponding to the Software Management Plan use case. For more information on SMPs see [ELIXIR Software Management Plan for Life Sciences](https://doi.org/10.37044/osf.io/k8znb). Properties have also been [mapped via crosswalks to other SMPs](https://doi.org/10.5281/zenodo.8087357). ",
      "rdfs:label": "SoftwareApplication",
      "rdfs:subClassOf": {
        "@id": "schema:SoftwareApplication"
      }
    },
    {
      "@id": "maSMP:SoftwareRunAction",
      "@type": "rdfs:Class",
      "rdfs:comment": "The act of testing an object according to its specifications. For instance, testing a software with a particular testType using a specific testInput and getting a specific testOutput (aka result).",
      "rdfs:label": "SoftwareRunAction",
      "rdfs:subClassOf": {
        "@id": "schema:Action"
      }
    },
    {
      "@id": "maSMP:SoftwareSourceCode",
      "@type": "rdfs:Class",
      "rdfs:comment": "Extension of schema:SoftwareSourceCode adding properties corresponding to the Software Management Plan use case. For more information on SMPs see [ELIXIR Software Management Plan for Life Sciences](https://doi.org/10.37044/osf.io/k8znb). Properties have also been [mapped via crosswalks to other SMPs](https://doi.org/10.5281/zenodo.8087357). ",
      "rdfs:label": "SoftwareSourceCode",
      "rdfs:subClassOf": {
        "@id": "schema:SoftwareSourceCode"
      }
    },
    {
      "@id": "maSMP:TestAction",
      "@type": "rdfs:Class",
      "rdfs:comment": "The act of testing an object according to its specifications. For instance, testing a software with a particular testType using a specific testInput and getting a specific testOutput (aka result).",
      "rdfs:label": "TestAction",
      "rdfs:subClassOf": {
        "@id": "schema:Action"
      }
    },
    {
      "@id": "maSMP:developerDocumentation",
      "@type": "rdf:Property",
      "schema:domainIncludes": [
        {
          "@id": "maSMP:SoftwareSourceCode"
        },
        {
          "@id": "maSMP:SoftwareApplication"
        }
      ],
      "schema:rangeIncludes": {
        "@id": "schema:CreativeWork"
      },
      "rdfs:comment": "Documentation about this software directed to developers who will use or reuse (e.g., extend) this software",
      "rdfs:label": "developerDocumentation"
    },
    {
      "@id": "maSMP:furtherDocumentation",
      "@type": "rdf:Property",
      "schema:domainIncludes": [
        {
          "@id": "maSMP:SoftwareSourceCode"
        },
        {
          "@id": "maSMP:SoftwareApplication"
        }
      ],
      "schema:rangeIncludes": {
        "@id": "schema:CreativeWork"
      },
      "rdfs:comment": "Any other documentation corresponding to this software that is not better specified by other documentation related properties",
      "rdfs:label": "furtherDocumentation"
    },
    {
      "@id": "maSMP:learningResource",
      "@type": "rdf:Property",
      "schema:domainIncludes": [
        {
          "@id": "maSMP:SoftwareSourceCode"
        },
        {
          "@id": "maSMP:SoftwareApplication"
        }
      ],
      "schema:rangeIncludes": {
        "@id": "schema:LearningResource"
      },
      "rdfs:comment": "Any [LearningResource](https://schema.org/LearningResource) that can provide orientation towards learning, education, skill acquisition, and other educational purposes about this research software.",
      "rdfs:label": "learningResource"
    },
    {
      "@id": "codemeta:referencePublication",
      "@type": "rdf:Property",
      "schema:domainIncludes": [
        {
          "@id": "maSMP:SoftwareSourceCode"
        },
        {
          "@id": "maSMP:SoftwareApplication"
        }
      ],
      "schema:rangeIncludes": {
        "@id": "schema:ScholarlyArticle"
      },
      "rdfs:comment": "An academic publication related to the software. Property defined in the [Codemeta terms](https://codemeta.github.io/terms/).",
      "rdfs:label": "referencePublication"
    },
    {
      "@id": "maSMP:runContainer",
      "@type": "rdf:Property",
      "schema:domainIncludes": {
        "@id": "maSMP:SoftwareRunAction"
      },
      "schema:rangeIncludes": {
        "@id": "schema:URL"
      },
      "rdfs:comment": "If the running was done using a container, such container should be pointed to here.",
      "rdfs:label": "runContainer"
    },
    {
      "@id": "maSMP:softwareRun",
      "@type": "rdf:Property",
      "schema:domainIncludes": {
        "@id": "maSMP:SoftwareRunAction"
      },
      "schema:rangeIncludes": [
        {
          "@id": "maSMP:SoftwareSourceCode"
        },
        {
          "@id": "maSMP:SoftwareApplication"
        }
      ],
      "rdfs:comment": "Software executed by this running action.",
      "rdfs:label": "softwareRun"
    },
    {
      "@id": "maSMP:softwareTested",
      "@type": "rdf:Property",
      "rdfs:comment": "Link to the software tested by this action.",
      "rdfs:label": "softwareTested",
      "schema:domainIncludes": {
        "@id": "maSMP:TestAction"
      },
      "schema:rangeIncludes": [
        {
          "@id": "schema:SoftwareSourceCode"
        },
        {
          "@id": "schema:SoftwareApplication"
        }
      ]
    },
    {
      "@id": "maSMP:testInput",
      "@type": "rdf:Property",
      "schema:domainIncludes": {
        "@id": "maSMP:TestAction"
      },
      "schema:rangeIncludes": [
        {
          "@id": "schema:Thing"
        },
        {
          "@id": "schema:ListItem"
        }
      ],
      "rdfs:comment": "Input used to performed the test. Some tests may not require any input, some may require multiple ones. If the order is important in the case of multiple inputs, a ListItem could help.",
      "rdfs:label": "testInput"
    },
    {
      "@id": "maSMP:testType",
      "@type": "rdf:Property",
      "schema:domainIncludes": {
        "@id": "maSMP:TestAction"
      },
      "schema:rangeIncludes": [
        {
          "@id": "schema:Text"
        },
        {
          "@id": "schema:URL"
        },
        {
          "@id": "schema:DefinedTerm"
        }
      ],
      "rdfs:comment": "The type of test that it is performed on the object.",
      "rdfs:label": "testType"
    },
    {
      "@id": "maSMP:testedWith",
      "@type": "rdf:Property",
      "schema:domainIncludes": [
        {
          "@id": "maSMP:SoftwareSourceCode"
        },
        {
          "@id": "maSMP:SoftwareApplication"
        }
      ],
      "schema:rangeIncludes": {
        "@id": "maSMP:TestAction"
      },
      "rdfs:comment": "Testing actions (e.g., continuous integration, end-to-end, etc.) performed on this software.",
      "rdfs:label": "testedWith"
    },
    {
      "@id": "maSMP:userDocumentation",
      "@type": "rdf:Property",
      "schema:domainIncludes": [
        {
          "@id": "maSMP:SoftwareSourceCode"
        },
        {
          "@id": "maSMP:SoftwareApplication"
        }
      ],
      "schema:rangeIncludes": {
        "@id": "schema:CreativeWork"
      },
      "rdfs:comment": "Documentation about this software directed to users who will use this software as it is.",
      "rdfs:label": "userDocumentation",
      "url": "https://github.com/MPDL/fedora-genericsearch-2.2/wiki"
    },
    {
      "@id": "maSMP:versionControlSystem",
      "@type": "rdf:Property",
      "schema:domainIncludes": {
        "@id": "maSMP:SoftwareSourceCode"
      },
      "schema:rangeIncludes": {
        "@id": "schema:SoftwareApplication"
      },
      "rdfs:comment": "Version control system used for this source code, to keep track of all commits, branches and so.",
      "rdfs:label": "versionControlSystem",
      "url": "https://github.com"
    }
  ]
}